\documentclass{article}
\usepackage{amsmath, amsthm, amsfonts, amssymb}
\usepackage{mathtools}
\usepackage{tikz-cd}
\usepackage{enumerate}
\usepackage[hidelinks]{hyperref}
\usepackage{cleveref}

\theoremstyle{plain}% default
\newtheorem{theorem}{Theorem}[section]
\newtheorem{lemma}{Lemma}[section]
\newtheorem{proposition}{Proposition}[section]
\newtheorem{remark}{Remark}[section]
\newtheorem{corollary}{Corollary}[section]

\theoremstyle{definition}
\newtheorem{definition}{Definition}[section]
\newtheorem{conjecture}{Conjecture}[section]
\newtheorem{example}{Example}[section]

\theoremstyle{remark}
\newtheorem*{note}{Note}
\newtheorem{case}{Case}
\newtheorem*{notation}{Notation}



\newcommand{\cob}{\mathcal{C}_\mathcal{O}^\bullet}
\newcommand{\co}{\mathcal{C}_\mathcal{O}}
\newcommand{\ann}{\operatorname{Ann}}
\newcommand{\im}{\operatorname{im}}
\newcommand{\fitt}{\operatorname{Fitt}}
\renewcommand{\hom}{\operatorname{Hom}}

\title{Fermat's Last Theorem}
\author{Josua Kugler}

\begin{document}
\maketitle
\tableofcontents
\section{Introduction}
\section{An Overview of Wiles' proof}
\newpage
\section{Wiles' numerical criterion}
Wiles has discovered a criterion for two rings in a specific category to be isomorphic that only depends on some numerical invariants
of these rings. The aim of this section is to prove that criterion in its purely algebraic form. 
%TODO: Explain how this fits into the rest of the proof.

\subsection{Preliminaries and examples}
Let \(\mathcal{O}\) be the ring of integers of a finite extension \(K\) of \(\mathbb Q_\ell\). 
As \(K\) is a local field, its ring of integers is a discrete valutation ring (DVR), i.e. 
\(\mathcal O\) is a local, noetherian Dedekind ring with maximal ideal \(\lambda\). 
It is complete with resp server usedect to the \(\lambda\)-adic topology, a principal ideal domain (PID) 
and has residue field \(k \coloneqq \mathcal{O}/\lambda\)  to name some properties that we will use in the course of the proof.

\(\mathbb Z_\ell\) is the ring of integers of \(\mathbb Q_\ell\) and \(\mathbb F_\ell = \mathbb Z_\ell/\ell \mathbb Z_\ell\) its residue field. 
As \(K/\mathbb{Q}_\ell\) is finite, the residue field of \(\mathcal{O}\) is a finite extension of $\mathbb F_\ell$ and therefore finite. 
%Not entirely clear to me

\paragraph{The categories \(\co\) and \(\cob\)}
In this section, we will mostly deal with very specific rings. Therefore we define the category \(\co\) where objects of \(\co\) are
local complete noetherian \(\mathcal O\)-algebras with residue field \(k\) and the morphisms are local \(\mathcal{O}\)-algebra morphisms.
Often, we even need some extra structure. 
We obtain the category \(\cob\) from \(\co\) by equipping an object \(A\) with an additional surjective map
\[\pi_A \colon A \twoheadrightarrow \mathcal{O},\]
the so-called augmentation map. Objects in \(\cob\) are often called \textit{augmented rings}.
The morphisms in \(\cob\) are local \(\mathcal{O}\)-algebra morphisms that respect the augmentation map structure, i.e. for a morphism
\(f \colon A \to B\) we have the commutative diagram
\[
\begin{tikzcd}[column sep=small]
    A \arrow[rr, "f"] \arrow [dr, "\pi_A", swap, twoheadrightarrow] & & B \arrow [dl, "\pi_B", twoheadrightarrow]\\
    & \mathcal{O} &
\end{tikzcd}.
\]

In order to state Wiles' criterion, we need some more definitions.
\begin{definition}
    \(A \in \co\) is \textit{finite flat}, if \(A\) is finitely generated and torsion-free as an \(\mathcal{O}\)-module.
    Note that \(\mathcal{O}\) is a PID and therefore being torsion-free is equivalent to being flat as an \(\mathcal{O}\)-module.
\end{definition}

\begin{definition}[complete intersection]
    A finite flat ring \(A \in \co\) is called a \textit{complete intersection}, if \(A\) is isomorphic as an \(\mathcal{O}\)-algebra
    to a quotient
    \[A \cong \mathcal{O}[[X_1, \dots, X_n]]/(f_1, \dots, f_n),\] where there are as many relations as there are variables.
    %Why is this a good definition? Where does the name come from? see probably remark 5.2
\end{definition}

Let's take a look at an example.
\begin{example}\label{ex:first_1}
    \(A = \{(a,b) \in \mathcal{O}\times\mathcal{O},\; a \equiv b\; (\operatorname{mod} \lambda^n)\} 
    \cong \mathcal{O}[[T]]/(T(T-\lambda^n))\) is a finite flat complete intersection in \(\cob\).
    The projection \(\pi_A\) is given by \(\pi_A(a,b) = a\).
    \begin{proof}
        Consider the map
        \begin{align*}
            \phi\colon \mathcal{O}[[T]]/(T(T-\lambda^n)) &\to A\\
            f &\mapsto (f(0), f(\lambda^n)).
        \end{align*}
        \subparagraph*{\(\phi\) is welldefined and respects the \(\mathcal{O}\)-algebra structure:}
        Let \(f_0\) be the constant term of a polynomial \(f\) and \(f_1 \coloneqq T^{-1}(f-f_0)\), s.t. \(f = f_0 + T\cdot f_1(T)\).
        Because of
        \[f(0) - f(\lambda^n) = (f_0 + 0\cdot f_1(0)) - (f_0 + \lambda^n \cdot f_1(\lambda^n)) = -\lambda^n \cdot f_1(\lambda^n),\]
        \(f(0) \equiv f(\lambda^n)\; (\operatorname{mod} \lambda^n)\) as required.
        Furthermore, \[\phi(T(T-\lambda^n)) = (0(-\lambda^n), \lambda^n(\lambda^n - \lambda^n)) = (0,0).\]
        Finally, we need to think about series in \(\mathcal{O}[[T]]\) with infinitely many terms.
        For the first component \(f(0)\) this doesn't matter, as \(\phi\) just takes the constant term. 
        As \(\mathcal{O}\) is complete with respect to the \(\lambda\)-adic topology, 
        the map \(\tilde\phi_2\colon \mathcal{O}[[T]] \to \mathcal{O},\; f \mapsto f(\lambda^n)\) is clearly welldefined and thus \(\phi\)
        is welldefined.
        %O-algebra structure:
        Let \(o \in \mathcal{O}\). Then 
        \[\phi(of) = ((of)(0),(of)(\lambda^n)) = (of(0), of(\lambda^n)) = o(f(0), f(\lambda^n)) = o\phi(f)\]
        \subparagraph*{Injectivity:}
        Let \(\phi(f) = 0\). Then \(f(0) = 0 \implies T | f\) and \(f(\lambda^n) = 0 \implies (T - \lambda) | f\).
        As a result, \(f \in T(T-\lambda)\).
        \subparagraph{Surjectivity:}
        Let \((a,b) \in A\).
        As \(a \equiv b \operatorname{mod} \lambda^n,\) we can write \(b = a + b' \cdot \lambda^n\). Because of
        \[\phi(\overline{a + b'T}) = (a, a + b' \lambda^n) = (a,b),\] \(\phi\) is surjective.
        \subparagraph*{\(A\in \cob\):}
        \(\mathcal{O}\) is noetherian, so \(\mathcal{O}[T]/(T(T-\lambda^n))\) is noetherian as well.
        \((\lambda, T)\) is a maximal ideal in \(\mathcal{O}[T]/(T(T-\lambda^n))\), because
        \[\left(\mathcal{O}[T]/(T(T-\lambda^n))\right)/(\lambda, T) = \mathcal{O}/(\lambda) = k.\]
        %Korollar 24.13 Alg II
        Therefore, the completion \(\mathcal{O}[T]/(T(T-\lambda^n))^{\wedge(\lambda, T)}\) 
        of \(\mathcal{O}[T]/(T(T-\lambda^n))\) with respect to \((\lambda, T)\) is a local ring with maximal ideal
        \(\widehat{(\lambda, T)}\).
        Consider the SES of finitely generated \(\mathcal{O}\)-modules
        \[
            0 \to (T(T - \lambda^n)) \mathcal{O}[T] \to \mathcal{O}[T] \to \mathcal{O}[T]/(T(T-\lambda^n)) \to 0.
        \]
        %Theorem 24.9
        As completion of finitely generated \(\mathcal{O}\)-modules is exact (because \(\mathcal{O}\) is noetherian), we get the SES
        \[
            0 \to (T(T-\lambda^n))\mathcal{O}[[T]] \to \mathcal{O}[[T]] \to \mathcal{O}[T]/(T(T-\lambda^n))^{\wedge (\lambda, T)}  \to 0.
        \]
        by completing with respect to \((\lambda, T)\).
        As a result, we have
        \[
            \mathcal{O}[T]/(T(T-\lambda^n))^{\wedge (\lambda, T)} = \mathcal{O}[[T]]/(T(T-\lambda^n)).
        \]
        As a result, \(\mathcal{O}[[T]]/(T(T-\lambda^n))\) is a local ring with maximal ideal \((\lambda, T)\).
        Therefore, its residue field is
        \[
            \mathcal{O}[[T]]/(T(T-\lambda^n))/(\lambda, T) = \mathcal{O}[T]/(T(T-\lambda^n))/(\lambda, T) = \mathcal{O}/(\lambda) = k.
        \]
        %Theorem 10.26 in Atiyah-MacDonald
        As \(\mathcal{O}[T]/(T(T-\lambda^n))\) is noetherian, its \((\lambda, T)\)-completion \(\mathcal{O}[[T]]/(T(T-\lambda^n))\)
        is again noetherian.

        In total, we get that \(A \cong \mathcal{O}[[T]]/(T(T-\lambda^n))\) is a local, complete, noetherian \(\mathcal{O}\)-algebra 
        with residue field \(k\; \implies A \in \co\). 
        \subparagraph{\(A\) is a finite flat complete intersection:}
        \(A\) is generated by \((1,1)\) and \(0, \lambda^n\) because
        \[
            (a,b) = a(1,1) + (0, \underbrace{b-a}_{\in \lambda^n}) = a(1,1) + c(0, \lambda^n).
        \]
        Also, \(A\) is torsion-free because \(\mathcal{O}\) is an integral domain. 
        As there is one variable and one relation in \(A \cong \mathcal{O}[[T]]/(T(T-\lambda^n))\), \(A\) is a complete intersection.
    \end{proof}
\end{example}

%probably add more examples

\begin{example}\label{ex:last_1}
    \(U = \mathcal{O}[[X_1, \dots, X_n]]\) with projection \(\pi_U\colon U \to \mathcal{O},\; f \mapsto f(0)\) lies in \(\cob\).
    \begin{proof}
        \(\mathcal{O}\) is noetherian, so \(\mathcal{O}[X_1, \dots, X_{n}]\) is noetherian as well.
        \((\lambda, X_1, \dots, X_n)\) is a maximal ideal in \(\mathcal{O}[X_1, \dots, X_n]\), because
        \[\left(\mathcal{O}[X_1, \dots, X_n]\right)/(\lambda, X_1, \dots, X_n) = \mathcal{O}/(\lambda) = k.\]
        %Korollar 24.13 Alg II
        Therefore, the completion \[\mathcal{O}[X_1, \dots, X_n]^{\wedge(\lambda, X_1, \dots, X_n)} = \mathcal{O}[[X_1, \dots, X_n]]\]
        of \(\mathcal{O}[X_1, \dots, X_n]\) with respect to \((\lambda, X_1, \dots, X_n)\) is a local ring with maximal ideal
        \(\widehat{(\lambda, X_1, \dots, X_n)}\).
        Its residue field is \(\mathcal{O}[X_1, \dots, X_n]/(\lambda, X_1, \dots, X_n) = k\), as required.
        As \(\mathcal{O}[X_1, \dots, X_n]\) is noetherian, its \((\lambda, X_1, \dots, X_n)\)-completion is again noetherian.
    \end{proof}
\end{example}

\begin{remark}
    In \cref{ex:first_1} we could write \(A\) as a quotient of \(\mathcal{O}[[X]]\). 
    This is possible in a more general setting, in fact every \(A \in \co\) can be written as a quotient of
    \(U = \mathcal{O}[[X_1, \dots, X_n]]\) for suitable \(n\).
\end{remark}
\begin{proof}
    As \(A\) is a noetherian ring and \(\ker \pi_A\) is an ideal in \(A\), it is finitely generated and therefore also finitely generated
    as an \(A\)-module. Consider the map
    \begin{align*}
        \Phi\colon U = \mathcal{O}[[X_1, \dots, X_n]] &\to A\\
        X_i &\mapsto a_i,
    \end{align*}
    where \(\ker \pi_A = (a_1, \dots, a_n)\) and \(\pi_U\) is given by \(f \mapsto f(0)\). 
    As \((X_1, \dots, X_n)\) generate the kernel of \(\pi_U\), this is a map in \(\cob\).
    We have the short exact sequences
    \[
        0 \to \ker \pi_A \to A \to \im \pi_A \cong \mathcal{O} \to 0
    \]
    and
    \[
        0 \to \ker \pi_U \to U \to \im \pi_U \cong \mathcal{O} \to 0
    \]
    As both corresponding sequences split via the inclusion \(\mathcal{O} \hookrightarrow A, x \mapsto x \cdot 1\)
    resp. \(\mathcal{O} \hookrightarrow U\), we can write \(A \cong \mathcal{O} \oplus \ker \pi_A\) 
    and \(A[[X_1, \dots, X_n]] \cong A \oplus \ker \pi_A\).
    \(\Phi\) by definition induces an equality on the first component, 
    a surjection on the second and therefore is surjective on the direct sum.
\end{proof}

\begin{definition}
    Let \(A \in \cob\). Then
    \[\phi_A \coloneqq (\ker \pi_A)/(\ker \pi_A)^2.\]
    %is the following helpful?
    The reader with background in algebraic geometry might notice that this can be though of as a tangent space, 
    in particular it is the cotangent space of the scheme \(\operatorname{spec}(A)\) at the point \(\ker \pi_A\).
    However this point of view is not necessary in the following, 
    it might be more a hint of how Wiles came to investigate this specific invariant.
\end{definition}

\begin{example}\label{ex:last_phi}
    Remember the definition of \(U\) in \cref{ex:last_1}.
    The tangent space \(\phi_U = \ker \pi_U/(\ker \pi_U)^2\) is
    \[
        \mathcal{O}X_1 \oplus \dots \oplus \mathcal{O}X_n.
    \]
    Indeed, elements of \(f \in \ker \pi_U\) have no constant term as \(f(0) = 0\) and therefore are multiples of \(X\).
    Elements in \(\ker \pi_U^2\) are multiples of \(X^2\). As a result, we receive elements \(\overline{f} \in \phi_U\) by
    cutting of all higher terms of a power series \(f \in \ker \pi_U\).
\end{example}

\begin{remark}
    Write \(A\) as a quotient of \(U,\; A = U/(f_1, \dots, f_n)\).
    We then get \(\phi_A = \phi_U/(\overline{f_1}, \dots, \overline{f_n})\).
    As a quotient of \(\phi_U\) its a finitely generated \(\mathcal{O}\)-module.
\end{remark}
\begin{proof}
    Consider the following map of \(\mathcal{O}\)-modules
    \begin{align*}
        \Phi\colon \ker \pi_U = \mathcal{O}X_1 \oplus \dots \oplus \mathcal{O}X_n &\to (\ker \pi_A)/(\ker \pi_A)^2 = \phi_A\\
        a_1X_1 + \dots + a_nX_n &\mapsto [a_1X_1 + \dots + a_nX_n] \; \mod (\ker \pi_A)^2,
    \end{align*}
    where \([f]\) denotes the image of \(f\) in \(A\).
    Then, as \(\pi_A([f]) = f(0)\), we get that \(X_i \in \ker \pi_A \forall i\)
    and therefore \([f] \in \ker \pi_A \forall f \in \ker \pi_U\). Not only is \(\Phi\) welldefined,
    we can conclude that \(X_i \in \ker \pi_A \implies X_i^2 \in (\ker \pi_A)^2\)
    and therefore \(\Phi\) is also surjective and \((\ker \pi_U)^2 \subset \ker \Phi\).
    
    With this knowledge we get a welldefined surjective map
    \begin{align*}
        \tilde \Phi\colon \phi_U &\to \phi_A\\
        a_1X_1 + \dots + a_nX_n \; \mod (\ker \pi_U)^2 &\mapsto [a_1X_1 + \dots + a_nX_n] \; \mod (\ker \pi_A)^2.
    \end{align*}
    Elements in the kernel of this map are either generated by \(X_i^2\) s.t. they become 0 \(\mod (\ker \pi_A)^2\)
    or they become 0 by sending them to \(A = U/(f_i)\).
    As higher order terms of \(f_i\) are vanishing anyways, 
    the kernel of \(\tilde \Phi\) is generated by the \(\overline{f_i}\), i.e.
    \[
        \phi_A \cong \phi_U/(\overline{f_i})  
    \]
\end{proof}

\begin{example}\label{ex:first_phi}
    We now compute \(\phi_A\) where \(A\) was defined in \cref{ex:first_1}.
    Remember that \(f = T(T-\lambda^n) = -\lambda^n T + T^2\). Therefore,
    \[\phi_A = \mathcal{O}T/(-\lambda^n T) = \mathcal{O}/\lambda^n.\]
\end{example}

\begin{definition}
    Let \(A \in \cob\). Then
    \[\eta_A \coloneqq \pi_A(\ann_A (\ker \pi_A))\] is an ideal in \(\mathcal{O}\).
\end{definition}

\begin{example}
    We now compute \(\eta_U\) for \(U\) from \cref{ex:last_1}.
    \begin{align*}
        \eta_U &= \pi_U(\ann \ker \pi_U)\\
        &= \pi_U(\ann \mathcal{O}X_1 \oplus \dots \oplus \mathcal{O}X_n)\\
        &= \pi_U(0) = 0.
    \end{align*}
\end{example}

\begin{lemma}\label{lem:ideals}
    Let \(\mathfrak a \subset \mathcal{O}\) be an ideal. Then
    \[\mathfrak a \neq 0 \implies \mathcal{O}/\mathfrak a \text{ finite}.\]
\end{lemma}
\begin{proof}
    As \(\mathcal{O}\) is a DVR, \(\mathfrak a = \lambda^n\) for some \(n \in \mathbb N\) 
    where \(\lambda\) is the maximal ideal in \(\mathcal{O}\).
    Therefore, \(\mathcal{O}/\mathfrak{a} = \mathcal{O}/\lambda^n.\)

    Using the fact that \(\lambda = (t)\) for some uniformizer \(t\), we get \(\forall i \ge 1\) 
    the isomorphism \(\lambda^i/\lambda^{i+1} \cong \mathcal{O}/\lambda = k\) and thereby also the short exact sequence 
    \[0 \to \mathcal{O}/\lambda \cong \lambda^i/\lambda^{i+1} \to \mathcal{O}/\lambda^{i+1} \to \mathcal{O}/\lambda^{i} \to 0.\]
    As \(k = \mathcal{O}/\lambda\) is finite, we can use induction
    \[\# \mathcal{O}/\lambda^{i+1} = \# \mathcal{O}/\lambda \cdot \# \mathcal{O}/\lambda^i = \# k \cdot (\# k)^i = (\# k)^{i+1}\]
    and get \(\# \mathcal{O}/\mathfrak{a} = \# \mathcal{O}/\lambda^n = (\# k)^n\).
\end{proof}

\begin{example}\label{ex:first_eta}
    We now compute \(\eta_A\) for \(A\) from \cref{ex:first_1}.
    \begin{align*}
        \eta_A &= \pi_A(\ann \ker \pi_A)\\
        &= \pi_A(\ann \{(0, b) \subset \mathcal{O}\times \mathcal{O} | b \equiv 0 \mod \lambda^n\})\\
        &= \pi_A(\{(a, 0) \subset \mathcal{O}\times \mathcal{O} | a \equiv 0 \mod \lambda^n\})\\
        &= \pi_A((\lambda^n) \times \mathcal{O})\\
        &= (\lambda^n)
    \end{align*}
\end{example}

With these results at hand, we can state 
\begin{theorem}[Wiles' numerical criterion]\label{thm:wiles_numerical_criterion}
    Let \(R \twoheadrightarrow T\) a surjective morphism of augmented rings, \(T\) finite flat and \(\eta_T \neq 0\) 
    (i.e. \(\mathcal{O}/\eta_T\) finite).
    Then the following are equivalent
    \begin{enumerate}[(a)]
        \item \(\# \phi_R \le \#(\mathcal{O}/\eta_T)\),
        \item \(\# \phi_R = \#(\mathcal{O}/\eta_T)\),
        \item \(R\) and \(T\) are complete intersections, and \(R \to T\) is an isomorphism.
    \end{enumerate}
\end{theorem}

\subsection{Basic properties of the invariants}
In this subsection we prove the equivalence (a) \(\Leftrightarrow\) (b) in \cref{thm:wiles_numerical_criterion}
by investigating the invariants \(\phi_A\) and \(\eta_A\) that we defined last section.

\begin{lemma}\label{lem:surjectivity_phi}
    A morphism \(f\colon A \to B \in \cob\) induces a homomorphism \(\phi_A \to \phi_B\) of \(\mathcal{O}\)-modules.
    This induced map is surjective if and only if the morphism \(A \to B\) is surjective.
\end{lemma}
\begin{proof}
    We have the commutative diagram
    \[
    \begin{tikzcd}[column sep=small]
        A \arrow[rr, "f"] \arrow [dr, "\pi_A", swap, twoheadrightarrow] & & B \arrow [dl, "\pi_B", twoheadrightarrow]\\
        & \mathcal{O} &
    \end{tikzcd}.
    \]
    It follows from the diagram that the restriction of \(f\) to \(\ker \phi_A\) maps to \(\ker \phi_B\),
    because \(\forall x \in \ker \phi_A\colon\; \pi_B(f(x)) = \pi_A(x) = 0\).
    Concatenating this with the projection to the tangent space, we get a map
    \[
        \tilde f\colon \ker \pi_A \to \ker \pi_B/(\ker \pi_B)^2 = \phi_B.
    \]
    In order to see that \(\tilde f\colon \phi_A \to \phi_B\) is welldefined, we need to show 
    \[
        f(\ker \pi_A)^2 \subset (\ker \pi_B)^2,
    \]
    however this follows from the fact that \(f(\ker \pi_A) \subset \ker \pi_B\) and that \(f\) is an algebra
    homomorphism:
    \[
        f(x^2) = \underbrace{f(x)}_{\in \ker \pi_B}\underbrace{f(x)}_{\in \ker \pi_B} \in (\ker \pi_B)^2 
    \]
    for any \(x \in \ker \pi_A\).

    First, let us assume that \(A \to B\) is a surjective map.
    In this case, every element \(x \in \ker \phi_B\) has a preimage in \(\ker \pi_A\). Indeed, \(\forall y \in f^{-1}(x)\subset A\colon\)
    \[
        \pi_A(y) = \pi_B(f(y)) = \pi_B(x) = 0.
    \]
    As a result, the induced map \(f\colon \ker \pi_A \to \ker \pi_B\) and its concatenation with
    the projection to \(\phi_B\), \(\tilde f\colon \ker \pi_A \to \ker \pi_B/(\ker \pi_B)^2\) are both surjective.
    In total, we obtain a surjective homomorphism \(\tilde f\colon \phi_A \to \phi_B\).
    
    Now, let the induced map \(\phi_A \to \phi_B\) be surjective. 

    %We know that \(\ker \pi_A\) is an ideal in \(A\), hence \(\ker \pi_A \subset \mathfrak{m}_A\).
    %As \(A\) is complete, we have \(A \cong \varprojlim A/\mathfrak{m}_A^n\).
    %Now consider the map
    %\[
    %    A \to \varprojlim A/(\ker \pi_A)^n = \hat A.
    %\]
    \textbf{Why is \(A\) complete with respect to the \(\ker \pi_A\)-adic topology?}
    Consider the ideal \(I = f(\ker \pi_A) \cdot B\) in \(B\).
    Let \(x \in I\). Then \(x = \sum_i f(x_i) \cdot b_i\) for \(x_i \in \ker \pi_A\) and \(b_i \in B\).
    Remember the commutative diagram from the beginning of the proof,
    \[
        \pi_B(x) = \pi_B\left(\sum_i f(x_i)\cdot b_i\right) = \sum_i \pi_B(f(x_i))\cdot \pi_B(b_i) = \sum_i\pi_A(x_i)\cdot \pi_B(b_i) = 0. 
    \]
    As a result, \(I \subset \ker \pi_B \subset \mathfrak{m}_B\).
    Note that
    \[f(\ker \pi_A) \subset f(\ker \pi_A)\cdot B \implies f((\ker \pi_A)^n) = f(\ker \pi_A)^n \subset (f(\ker \pi_A)\cdot B)^n,\]
    so we have \(\phi((\ker \pi_A)^n)\cdot B \subset I^n\).
    As \(B\) is \(\mathfrak{m}_B\)-adically complete and therefore Hausdorff, we get
    \[
        \bigcap_{n \in \mathbb N} f((\ker \pi_A)^n) \cdot B \subset \bigcap_{n \in \mathbb N} I^n 
        \subset \bigcap_{n \in \mathbb N} \mathfrak{m}_b^n = 0,
    \]
    i.e. \(\!B\) is separated with respect to the \(I\)-adic topology.
    Furthermore, \(\ker \pi_A\) is finitely generated as an \(A\)-module, \(\ker \pi_A = \langle a_1, \dots, a_m\rangle\) because \(A\) is noetherian. 
    As \(\ker \pi_A \to (\ker \pi_B)/(\ker \pi_B)^2\) is surjective, we have 
    \[(\ker \pi_B)/(\ker \pi_B)^2 = \langle \overline{f(a_1)}, \dots, \overline{f(a_m)}\rangle_B.\]
    \textbf{As \(A\) is complete} and \(I\) is separated with respect to the \(I\)-adic topology as a submodule of \(B\), 
    we can apply Nakayama's Lemma as in Mat, 8.4. It follows that the images \(\langle f(a_1), \dots, f(a_m)\rangle\) generate \(\ker \pi_B\)
    as a \(B\)-module. We already know that \(f(\ker \pi_A) \cdot B \subset \ker \pi_B\). Together we have
    \[
        f(\ker \pi_A) \cdot B = \ker \pi_B.
    \]
    Now we conclude that \(1\) is a generator of \(B/I = B/f(\ker \pi_A) B = B/\ker \pi_B = \mathcal{O}\) as an 
    \(A/\ker \pi_A \cong \mathcal{O}\)-module.
    Applying Nakayama's Lemma again, we get that \(1\) is a generator of \(B\) as an \(A\)-module and hence, \(f\colon A \to B\) is surjective.
\end{proof}

\begin{corollary}\label{cor:surjectivity_phi}
    \(A \to B\) is surjective if and only if \[\phi_A \geq \phi_B.\]
\end{corollary}

\begin{lemma}
    If \(f \colon A \to B\) is surjective, then
    \begin{equation}
        \eta_A \subset \eta_B, \quad \text{i.e.,}\quad \#(\mathcal{O}/\eta_A) \geq \#(\mathcal{O}/\eta_B).  
    \end{equation}
\end{lemma}
\begin{proof}
    As we have seen in the proof of \cref{lem:surjectivity_phi}, a surjective map \(f\) induces a surjective
    map on the kernels, \(f\colon \ker \pi_A \to \ker\pi_B\).
    Now let \(x \in \ann_A \ker \pi_A\), i.e. \(x \cdot a = 0\;\; \forall a \in \ker \pi_A\).
    For all \(b \in \ker \pi_B\) and any preimage \(a \in \ker \pi_A\) we have
    \[
        f(x) \cdot b = f(x) \cdot f(a) = f(x \cdot a) = f(0) = 0.
    \]
    As a result, \(f(x) \in \ann_B\ker \pi_B\) and we obtain a map
    \[
        \tilde f\colon\ann_A\ker \pi_A \to \ann_B \ker \pi_B.  
    \]
    In order to show \(\eta_A \subset \eta_B\), let \(x \in \eta_A = \pi_A(\ann_A \ker \pi_A)\), i.e.
    \(x = \pi_A(y)\) for some \(y \in \ann_A \ker \pi_A\). By the commutative diagram
    \[
    \begin{tikzcd}[column sep=small]
        \ann_A \ker \pi_A \arrow[rr, "\tilde f"] \arrow [dr, "\pi_A", swap, twoheadrightarrow] 
        & & \ann_B \ker \pi_B \arrow [dl, "\pi_B", twoheadrightarrow]\\
        & \mathcal{O} &
    \end{tikzcd},
    \]
    we get
    \[
        x = \pi_A(y) = \pi_B(\tilde f(y)) \in \pi_B(\ann_B \ker \pi_B) \implies x \in \eta_B,
    \]
    as desired.
\end{proof}

%TODO: insert some remarks on Fitting ideals
\begin{definition}
    Let \(M\) be a finitely generated \(R\)-module. Then \(M\) is a quotient
    \[
        P \colon R^n \longrightarrow M = R^n/\ker P
    \]
    We define \(\fitt_R(M) \coloneqq \langle \det(v_1, \dots, v_n) | v_i \in \ker P \rangle_R \subset R\).
    This is independent of the choice of the surjection (see e.g. stacks project).
\end{definition}

\begin{lemma}\label{lem:fitting_and_ann}
    For a finitely generated \(R\)-module \(M\) we have
    \[\fitt_R(M) \subset \ann_R(M).\]
\end{lemma}
\begin{proof}
    \(M\) is generated by \(\overline{e_1}, \dots, \overline{e_n}\) where \(\overline{x}\) 
    may denote the residue class of \(x \mod \ker P\).
    Now let \([v_1|\dots|v_n]\) be a matrix with \(v_i \in \ker P\). Then this matrix annihilates \(M\) because
    it annihilates all the generators \(\overline{e_i}\),
    \[
        [v_1|\dots|v_n] \cdot e_i = v_i \in \ker P.
    \]
    Let \(A\) be the adjugate matrix of \([v_1|\dots|v_n]\), i.e. \[A[v_1|\dots|v_n] = \det [v_1|\dots|v_n]\cdot I_{n\times n}.\]
    Let \(m \in M\) and \((m_i)_{i=1}^n\) a lift in \(R^n\). Then we have 
    \begin{align*}
        \det [v_1|\dots|v_n] \cdot m &= \det [v_1|\dots|v_n]\cdot I_{n\times n} (m_i)_{i=1}^n \\
        &= A[v_1|\dots|v_n]\left(\sum_{i=1}^n m_i e_i\right)\\
        &= A \cdot \sum_{i=1}^n m_i v_i \in A \cdot \ker P \subset \ker P
    \end{align*}
    Therefore \(\fitt_R(M) \subset \ann_R(M)\).
\end{proof}

\begin{remark}[Fitting ideals and \(\otimes\)]\label{rem:fitting_and_tensor}
    Let \(A \in \cob\) and \(M\) a finitely generated \(A\)-module. 
    Note that \(\mathcal{O}\) has an \(A\)-module structure via \(\pi_A\).
    We have
    \[
        \pi_A(\fitt_A(M)) = \fitt_\mathcal{O}(M \otimes_A \mathcal{O}).
    \]
    This follows from the fact that \(- \otimes_A \mathcal{O}\) is right exact. 
    Hence, from the exact sequence
    \[
        \ker P \longrightarrow A^n \longrightarrow M \longrightarrow 0
    \]
    we get the exact sequence
    \[
        \ker P \otimes_A \mathcal{O} \longrightarrow A^n\otimes_A \mathcal{O} = \mathcal{O}^n 
        \longrightarrow M\otimes_A \mathcal{O} \longrightarrow 0.
    \]
    The remaining details are left as an exercise to the reader.
\end{remark}

\begin{remark}[Fitting ideals for finitely generated \(O\)-modules]
    Let \(M\) be a finitely generated \(O\)-module. As \(O\) is a PID, there are unique \(r,s \in \mathbb{N}\) 
    and \(n_1 \geq dots \geq n_s \in \mathbb{N}\) s.t.
    \[
        M = \mathcal{O}^r \oplus \mathcal{O}/\lambda^{n_1} \oplus \dots \oplus \mathcal{O}/\lambda^{n_s}.
    \]
    If \(r > 0\) then every \(v \in \ker P \subset \mathcal{O}^{r + s}\) has \(r\) zero components.
    Therefore, \(\fitt_R (M) = 0\) for \(r > 0\).
    If \(r = 0\) the \(i\)-th component of \(v \in \ker P \subset \mathcal{O}^s\) 
    lies in the kernel of \(\mathcal{O} \to \mathcal{O}/\lambda^{n_i}\), 
    i.e. \(v_i \in \lambda^{n_i}\).
    Using the Leibniz formula for computing the determinant, we get
    \(\fitt_\mathcal{O}(M) = \lambda^{n_1} \cdot \dots \cdot \lambda^{n_s} = \lambda^{n_1 + \dots + n_s}\).
\end{remark}

\begin{corollary}\label{cor:fitting_finite}
    Let \(M\) be a finite \(\mathcal{O}\)-module. Then
    \[
        \# M = \# (\mathcal{O}/\fitt_\mathcal{O}(M)). 
    \]
\end{corollary}
\begin{proof}
    As \(M\) is finite, we get
    \[
        M = \mathcal{O}/\lambda^{n_1} \oplus \dots \oplus \mathcal{O}/\lambda^{n_s}
    \]
    and 
    \[
        \fitt_\mathcal{O}(M) = \lambda^{n_1 + \dots + n_s}.
    \]
    From the proof of \cref{lem:ideals} it follows that
    \[\# M = (\# k)^{n_1} \cdot \dots \cdot (\# k)^{n_s} = (\# k)^{n_1 + \dots + n_s}\]
    and
    \[
        \# (\mathcal{O}/\fitt_\mathcal{O}(M)) = \# (\mathcal{O}/\lambda^{n_1 + \dots + n_s}) = (\# k)^{n_1 + \dots + n_s}.
    \]
\end{proof}

\begin{lemma}\label{lem:standard_ineq}
    Let \(A \in \co\). Then \[\#\phi_A \geq \#(\mathcal{O}/\eta_A).\]
\end{lemma}
\begin{proof}
    As \(\mathcal{O} = A/\ker \pi_A\), we have
    \[
        \ker \pi_A \otimes_A \mathcal{O} = \ker \pi_A \otimes_A A/\ker \pi_A \cong \ker \pi_A/(\ker \pi_A) \ker \pi_A = \phi_A.
    \]
    We therefore have
    \[
        \fitt_\mathcal{O}(\phi_A) = \fitt_\mathcal{O}(\ker \pi_A \otimes_A\mathcal{O}) = \pi_A(\fitt_A(\ker \pi_A))
    \]
    where the second equality follows from \cref{rem:fitting_and_tensor}.
    Applying \cref{lem:fitting_and_ann} to the RHS, we get 
    \[
        \fitt_\mathcal{O}(\phi_A) \subset \pi_A(\ann_A(\ker \pi_A)) = \eta_A.
    \]
    \textbf{Why is \(\phi_A\) finite?}
    As \(\phi_A\) is finite, we can apply \cref{cor:fitting_finite} to \(M = \phi_A\) and obtain
    \[
        \# \phi_A = \# (\mathcal{O}/\fitt_\mathcal{O}(\phi_A)) \geq \# (\mathcal{O}/\eta_A).
    \]
\end{proof}

\begin{proposition}
    (a) \(\Leftrightarrow\) (b) in \cref{thm:wiles_numerical_criterion}.
\end{proposition}
\begin{proof}
    By assumption, \(R \to T\) is a surjective morphism in \(\cob\).
    With \cref{cor:surjectivity_phi} it follows that \(\#\phi_R \geq \#\phi_T\).
    \cref{lem:standard_ineq} tells us that \(\#\phi_T \geq \#(\mathcal{O}/\eta_T)\).
    The inequalities combine to \[\#\phi_R \geq \#(\mathcal{O}/\eta_T).\]
    \begin{itemize}
        \item[(a)\(\implies\)(b)] (a) gives us \(\#\phi_R \leq \#(\mathcal{O}/\eta_T)\), so combined with the 
        inequality \(\#\phi_R \geq \#(\mathcal{O}/\eta_T)\) we have just proven we conclude that (b) must hold.
        \item[(b)\(\implies\)(a)] Obvious.
    \end{itemize}      
\end{proof}

\subsection{Regular sequences and the Koszul complex}
Let \(A\) be a finite flat complete intersection. Hence we can write 
\[A = \mathcal{O}[[X_1, \dots, X_n]]/(f_1, \dots, f_n).\]
The goal of this section is to prove some technical lemmata and to introduce
the Koszul complex that we will use to construct two \(\mathcal{O}[[X]]\)-free resolutions for \(A\).
This will turn out to be crucial in the next section.

We start with a few definitions from commutative algebra.
\begin{definition}[primary ideal]
    Let \(R\) be a local ring and \(\mathfrak{a} \subsetneq R\) an ideal. 
    \(\mathfrak{a}\) is said to be primary if every zero divisor in \(R/\mathfrak{a}\) is nilpotent.
\end{definition}
Recall that the dimension of a ring is given by
\[
    \sup \left\{n | 
                \mathfrak{p}_0 \subsetneq \dots \subsetneq \mathfrak{p}_n \subsetneq R,\; \mathfrak{p}_i \text{ prime} 
        \right\}.
\]
\begin{definition}[system of parameters]
    Let \(x_1, \dots, x_n\) generate a primary ideal of \(R\). If \(n = \dim R\) then \(x_1, \dots, x_n\) is called 
    a system of parameters.
\end{definition}

\begin{definition}[regular sequence]
    A sequence \((x_1, \dots, x_n)\) is said to be a regular sequence 
    if \(\forall\; i = 1, \dots, n\colon\)
    \[x_i \text{ is not a zero-divisor in } R/(x_1, \dots, x_{i-1}).\]
\end{definition}

\begin{lemma}
    The sequence \((f_1, \dots, f_n, \lambda)\) is a system of parameters for \(U\) (cf. \cref{ex:last_1}).
\end{lemma}
\begin{proof}
    First, we show that \(\dim U = n + 1\).
    We have an ascending chain of prime ideals
    \[
        (0) \subsetneq (\lambda) \subsetneq \dots \subsetneq (\lambda, X_1, \dots, X_n),  
    \]
    so by definition of the dimension we get \(\dim U \geq n + 1\).
    %Corollary 26.18 of Prof. Schmidt's Algebra script
    Let \(\mathfrak{m} = (\lambda, X_1, \dots, X_n)\). We have seen that this is the maximal ideal in \(U\).
    Now we can conclude
    \[
        \dim U \leq \dim_{U/\mathfrak{m}}(\mathfrak{m}/\mathfrak{m}^2) 
        = \dim_k(\lambda/\lambda^2 \oplus k X_1 \oplus \dots \oplus k X_n).
    \]
    As \(\lambda/\lambda^2 \cong k\) (cf. \cref{lem:ideals}), the above expression evaluates to \(n+1\) and
    taking both inequalities together we obtain \(\dim U = n + 1\).
    It remains to show that \((f_1, \dots, f_n, \lambda)\) generate a primary ideal of \(U\).
    \(U\) is local and therefore the quotient ring 
    \[\tilde{U} \coloneqq U/(f_1, \dots, f_n, \lambda)\] 
    is local as well.
    Also, \(\tilde U\) is a \(k\)-vector space (because it's an \(\mathcal{O}\)-module and \(\lambda\)-operation
    annihilates it). As \(A = U/(f_1, \dots, f_n)\) is a finitely generated \(\mathcal{O}\)-module, we can find
    \((x_1, \dots, x_N)\) that generate \(A\) as \(\mathcal{O}\)-module.
    These \(x_i\) then generate \(\tilde U\) as a \(k\)-vector space.
    Every element in the maximal ideal of \(\tilde U\) is nilpotent \textbf{because ??}
\end{proof}

\begin{lemma}\label{lem:reg_seq}
    The sequence \((f_1, \dots, f_n)\) is a regular sequence for \(U\).
\end{lemma}
\begin{proof}
    The sequence \((\lambda, X_1, \dots, X_n)\) is a regular sequence for \(U\) because
    \(U/\lambda = k[[X_1, \dots, X_n]]\) and \(U/(\lambda, X_1, \dots, X_{i-1}) = k[[X_i, \dots, X_n]]\) 
    are integral domains (hence obviously \(X_i\) can't be a zero-divisor in these rings).
    As we have seen in the previous lemma, it's as well a system of parameters.
    Therefore, the depth of \(U\) (i.e. the maximal lenth of any regular sequence in \(U\)) is bigger than
    the length of the particular regular sequence \((\lambda, X_1, \dots, X_n)\).
    In total we get \(\operatorname{depth} U \geq \dim U\), because \((\lambda, X_1, \dots, X_n)\) 
    is a system of parameters as well.
    %source?
    In general, we have \(\operatorname{depth} R \leq \dim R\) for a noetherian local ring \(R\), 
    so combined we have
    \[
        \operatorname{depth} U = \dim U  
    \]
    and hence, \(U\) is Cohen-Macaulay.
    %Matsumura, Theorem 17.4
    As \((f_1, \dots, f_n, \lambda)\) is a system of parameters and \(U\) is Cohen-Macaulay
    it follows by [Matsumura, Theorem 17.4] that \((f_1, \dots, f_n, \lambda)\) is a regular sequence.
    A fortiori, the sequence \((f_1, \dots, f_n)\) is also a regular sequence.
\end{proof}

\subsection{Complete intersections and the Gorenstein condition}
Let \(A\) be a finite flat complete intersection in \(\cob\). The goal of this section is to show that \(A\)
satisfies a Gorenstein condition, i.e. a specific form of self-duality.
This fact can then be used to show (c) \(\implies\) (b) in \cref{thm:wiles_numerical_criterion}.
Although there is a very general notion of Gorenstein rings, for
the purpose of this proof we only need a special case,
\begin{definition}
    Let \(A \in \co\) be finite flat. \(A\) is called Gorenstein, if there is an isomorphism of \(A\)-modules
    \[
        \Psi\colon \hom_\mathcal{O}(A, \mathcal{O}) \cong A.
    \]
\end{definition}

Our goal therefore reduces to constructing an \(A\)-module isomorphism
\[
    \hom_\mathcal{O}(A, \mathcal{O}) \to A.
\]

We start with some useful constructions and conventions.
\begin{notation}
    For any ring \(R\) write \(R[[\underline{X}]] \coloneqq R[[X_1, \dots, X_n]]\).
\end{notation}

Let \(a_1, \dots, a_n\) be the images in \(A\) of \(X_1, \dots, X_n\) by the natural map
\[
    \alpha \colon \mathcal{O}[[\underline{X}]] \to A = \mathcal{O}[[\underline{X}]]/(f_1, \dots, f_n),
\]
and let
\[
    \beta \colon A[[\underline{X}]] \to A  
\]
be the natural map which sends \(X_i\) to \(a_i\). The sequence \(g_i =  (X_i - a_i)\) 
generates the kernel of \(\beta\). \textbf{Why?}
View the \(f_i\) as polynomials in \(A[[\underline{X}]]\) via the inclusion \(O \hookrightarrow A\). Then \(\forall i = 1, \dots, n\colon\)
\[
    \beta(f_i) = f_i(a_1, \dots, a_n) = 0 \in \mathcal{O}[[\underline{X}]]/(f_1, \dots, f_n).
\]
Therefore every of the \(f_i\) is element of \(\ker \beta\) and hence can be written as 
an \(A[[X]]\)-linear combination of the \(g_i\),
\[
    (f_1, \dots, f_n) = (g_1, \dots, g_n)M,  
\]
where \(M\) is an \(n \times n\) matrix with coefficients in \(A[[\underline{X}]]\). 
Let \(D = \det(M) \in A[[\underline{X}]]\).

%unnecessary:
%We begin by constructing a surjective (\(\mathcal{O}\)-linear) map
%\[
%    \hom_\mathcal{O}[[\underline{X}]](A[[\underline{X}]], \mathcal{O}[[\underline{X}]]) \to A.
%\]

The projection \(\mathcal{O}[[\underline{X}]] \to A\) induces an \(\mathcal{O}[[\underline{X}]]\)-module 
structure on \(A\).

\begin{lemma}
    The map
    \begin{align*}
        \Phi\colon \hom_\mathcal{O}[[\underline{X}]](A[[\underline{X}]], \mathcal{O}[[\underline{x}]]) &\to A\\
        f &\mapsto \alpha(f(D))
    \end{align*}
    is an \(\mathcal{O}[[\underline{X}]]\)-linear surjection.
\end{lemma}
\begin{proof}
    As shown in \cref{lem:reg_seq}, \((\underline{f}) = (f_1, \dots, f_n)\) 
    is a regular sequence for \(\mathcal{O}[[\underline{X}]]\).
    In the ring \(A[[\underline{X}]]/(X_1 - a_1, \dots, X_{i-1} - a_{i-1})\), there are no relations in \(X_i\),
    i.e. it can be written as \(R[X_i]\) for a ring \(R\). Therefore \((X_i - a_i)\) can't be a zero-divisor.
    As this holds for all \(i = 1, \dots, n\), \((\underline{g}) = (g_i) = (X_i - a_i)\) is a regular sequence 
    for \(A[[\underline{X}]]\).
    
    Let now \(K(\underline{f}, \mathcal{O}[[\underline{X}]])\) and \(K(\underline{g}, A[[\underline{X}]])\)
    be the associated Koszul complexes. 
    %Koszul complex property 1:
    We have that \(K(\underline{f}, \mathcal{O}[[\underline{X}]])\) is a resolution of 
    \[
        A = H_0(\underline{f}, \mathcal{O}[[\underline{X}]]) = \mathcal{O}[[\underline{X}]]/(f_1, \dots, f_n)
    \]
    by free \(\mathcal{O}[[\underline{X}]]\)-modules
    and analogous that \(K(\underline{g}, A[[\underline{X}]])\) is a resolution of
    \[
        A = H_0(\underline{g}, A[[\underline{X}]]) = A[[\underline{X}]]/(X_1 - a_1, \dots, X_n-a_n)
    \]
    by free \(A[[\underline{X}]]\)-modules.
    Every free \(A[[\underline{X}]]\)-module has a canonical \(\mathcal{O}[[\underline{X}]]\)-module structure 
    (take the canonical inclusion \(\mathcal{O} \hookrightarrow A, x \mapsto x\cdot 1\) and extend it to a map
    \(\mathcal{O}[[\underline{X}]] \hookrightarrow A[[\underline{X}]]\)).

    In the following, we want to construct a map of complexes
    \[\Phi\colon K(\underline{f}, \mathcal{O}[[\underline{X}]]) \to K(\underline{g}, A[[\underline{X}]]).\]
    On the 0-th level, we define 
    \[
        \phi_0 \colon K_0(\underline{f}, \mathcal{O}[[\underline{X}]]) = \mathcal{O}[[\underline{X}]] 
        \to 
        K_0(\underline{g}, A[[\underline{X}]]) = A[[\underline{X}]]
    \]
    to be just the canonical inclusion \(\mathcal{O}[[\underline{X}]] \hookrightarrow A[[\underline{X}]]\)
    as explained above.
    %Koszul complex property 2:
    On the first level, let
    \[
        \Phi_1 \colon 
            K_1(\underline{f}, \mathcal{O}[[\underline{X}]]) = \bigoplus_{i = 1}^n R \cdot u_i
            \to 
            K_1(\underline{g}, A[[\underline{X}]]) = \bigoplus_{i=1}^n R \cdot v_i
    \]
    be the map defined by
    \[
        (\Phi_1(u_1), \dots, \Phi_1(u_n)) = (v_1, \dots, v_n)M. %probably explain this in greater detail
    \]
    By skew-linearity this can be extended to a map of exterior algebras. %What exactly is an exterior algebra?
    %Check the following facts
    %- this is a map of complexes
    %- it induces the identity map A -> A
    %- it satisfies phi(u_1 /\ ... /\ u_n) = D (v_1 /\ ... /\ v_n)
    In the following we proof that \(\Phi\)
    \begin{enumerate}
        \item is a morphism of complexes,
        \item induces the identity on \(A = H_0(\underline{f}, \mathcal{O}[[\underline{X}]])\)
        \item and satisfies
        \[
            \Phi_n(u_1 \wedge \dots \wedge u_n) = D \cdot v_1 \wedge \dots \wedge v_n.  
        \]
    \end{enumerate}
    \begin{enumerate}
        \item \textbf{\(\Phi\) is a morphism of complexes.}
        It is clear by definition that \(\Phi\) is welldefined on every level.
        We have to show that \(\Phi\) commutes with the differentials of the complex,
        \begin{align*}
            \Phi_{p-1}(d(u_{i_1}\!\wedge\!\dots\!\wedge\!u_{i_p})) 
            &= \Phi_{p-1}\left(\sum_{t=1}^p(-1)^t x_{i_t} 
            u_{i_1}\!\wedge\!\dots\!\wedge\!\widehat{u_{i_t}}\!\wedge\!\dots\!\wedge\!u_{i_p}\right)\\
            &= \sum_{t=1}^p(-1)^t x_{i_t}\Phi_1(u_{i_1})\!\wedge\!\dots\!
            \wedge\widehat{\Phi_1(u_{i_t})}\!\wedge\!\dots\!\wedge\!\Phi_1(u_{i_p})\\
            &= d(\Phi_1(u_{i_1})\wedge\dots\wedge \Phi_1(u_{i_p}))\\
            &= d(\Phi_p(u_{i_1}\wedge\dots\wedge u_{i_p})).
        \end{align*}
        \item \textbf{\(\Phi\) induces the identity on \(A = H_0(\underline{f}, \mathcal{O}[[\underline{X}]])\)}\\
        We have the following commutative diagram
        \[
            \begin{tikzcd}
                \bigoplus_{i=1}^n u_i \mathcal{O}[[\underline{X}]] = K_1(\underline{f}, \mathcal{O}[[\underline{X}]]) 
                \arrow[r, "d_1"] \arrow[d, "\Phi_1"] & K_0(\underline{f}, \mathcal{O}[[\underline{X}]]) \arrow[r, "d_0"] \arrow[d, hook, "\Phi_0"] = \mathcal{O}[[\underline{X}]] & 0\\
                \bigoplus_{i=1}^n v_i A[[\underline{X}]] = K_1(\underline{g}, A[[\underline{X}]]) 
                \arrow[r, "d_1"] & K_0(\underline{g}, A[[\underline{X}]]) = A[[\underline{X}]] \arrow[r, "d_0"] & 0
            \end{tikzcd}.
        \]
        As 
        \[
            H_0(\underline{f}, \mathcal{O}[[\underline{X}]]) = \frac{\ker d_0}{\im d_1} 
            = \frac{\mathcal{O}[[\underline{X}]]}{(f_1, \dots, f_n)}
        \] and
        \[
            H_0(\underline{g}, A[[\underline{X}]]) = \frac{\ker d_0}{\im d_1} 
            = \frac{A[[\underline{X}]]}{(g_1, \dots, g_n)}
        \]
        we can take a look at the map
        \[
            \mathcal{O}[[\underline{X}]] \to \frac{A[[\underline{X}]]}{(X_1 - a_1, \dots, X_n - a_n)} = A.
        \]
        This map sends \(X_i\) to \(a_i \in A\).
        By definition of \(A = \mathcal{O}[[\underline{X}]]/(f_1, \dots, f_n)\) and \(a_i\) as image of \(X_i\)
        under \(\alpha\) this is exactly the map \(\alpha\). \textbf{Really?} Hence, the induced map
        \[
            A = \mathcal{O}[[\underline{X}]]/(f_1, \dots, f_n) \to 
            \frac{A[[\underline{X}]]}{(X_1 - a_1, \dots, X_n - a_n)} = A
        \]
        is identity.
        \item Let \(M = (M_{i,j})_{i,j}\). Then we have
        \begin{align*}
            \Phi_n(u_1 \wedge \dots \wedge u_n) &= \Phi(u_1) \wedge \dots \wedge \Phi(u_n)\\
            &= \sum_{j=1}^n v_jM_{j,1} \wedge \dots \wedge \sum_{j=1}^n v_jM_{j,n}\\
            &= \underbrace{\sum_{\sigma \in \mathfrak{S}(n)} (-1)^{\operatorname{sgn}(\sigma)} \prod_{i=1}^n M_{i,\sigma(i)}}_{= \det M} \cdot v_1 \wedge \dots \wedge v_n\\
            &= D \cdot v_1 \wedge \dots \wedge v_n,
        \end{align*}
        where \(\mathfrak{S}(n)\) may denote the group of permutations.
    \end{enumerate}
    In the following we write 
    \(K^\bullet(\underline{f}) = K^\bullet(\underline{f}, \mathcal{O}[[\underline{X}]])\)
    and 
    \(K^\bullet(\underline{g}) = K^\bullet(\underline{g}, A[[\underline{X}]])\)
    By applying the functor \(\hom_{\mathcal{O}[[\underline{X}]]}(-, \mathcal{O}[[\underline{X}]])\)
    to the two free resolutions, we get the following commutative diagram
    \[
        \begin{tikzcd}[column sep=2.2em]
            \arrow[r, "d_{n-1}^*"] & 
            \hom_{\mathcal{O}[[\underline{X}]]}(K^{n-1}(\underline{f}), \mathcal{O}[[\underline{X}]]) 
            \arrow[r, "d_n^*"] &
            \hom_{\mathcal{O}[[\underline{X}]]}(K^n(\underline{f}), \mathcal{O}[[\underline{X}]]) 
            \arrow[r] & 0\\
            \arrow[r, "d_{n-1}^*"] & 
            \hom_{\mathcal{O}[[\underline{X}]]}(K^{n-1}(\underline{g}), \mathcal{O}[[\underline{X}]])
            \arrow[r, "d_n^*"] \arrow[u, "\Phi_{n-1}^*"] &
            \hom_{\mathcal{O}[[\underline{X}]]}(K^n(\underline{g}), \mathcal{O}[[\underline{X}]]) 
            \arrow[r] \arrow[u, "\Phi_{n}^*"] & 0
        \end{tikzcd}.
    \]
    \textbf{Here comes the argumentation why \(Phi\) is a homotopy equivalence}
    Hence, we have an isomorphism on the \(n\)-th cohomology,
    \[
        \Phi_n*\colon \hom_{\mathcal{O}[[\underline{X}]]}(K^n(\underline{g}), \mathcal{O}[[\underline{X}]]) 
        \to \hom_{\mathcal{O}[[\underline{X}]]}(K^n(\underline{f}), \mathcal{O}[[\underline{X}]]).
    \]
    We know that \(H_n(\underline{g})\cong\)
\end{proof}

\end{document}