\begin{frame}
\begin{block}{Beweis.}
    \begin{align*}
        \pi^{-s/2} \Gamma(s/2)\zeta(s) &= \alt<1>{\sum_{n = 1}^{\infty} \int_0^\infty}{\int_0^\infty \sum_{n = 1}^{\infty}} e^{-\pi n^2 t}t^{s/2} \frac{\intd t}{t}\\
        \visible<3->{&= \int_0^\infty \frac{\theta(it)-1}{2} t^{s/2} \frac{\intd t}{t}\\}
        \visible<4->{&= \underbrace{\int_0^1 \frac{\theta(it)-1}{2} t^{s/2} \frac{\intd t}{t}}_{R_0(s)} + \underbrace{\int_1^\infty \frac{\theta(it)-1}{2} t^{s/2} \frac{\intd t}{t}}_{R_\infty(s)}\\}
        \visible<5->{&= R_0(s) + R_\infty(s)}
    \end{align*}
\end{block}
\end{frame}
