\begin{frame}[t]
    \begin{proof}
    \begin{align*}%geometrische Reihe
        \visible<6->{\lim\limits_{m \to \infty}}\visible<2->{\prod_{k=1}^m} \frac{1}{1-p_k^{-s}} &= \only<6->{\lim\limits_{m \to \infty}}\only<2->{\prod_{k=1}^m} \sum_{\nu = 0}^\infty \frac{1}{p_k^{\nu s}}\only<3>{\scriptscriptstyle =\left(1 + \frac{1}{p_1^s} + \frac{1}{p_1^{2s}} \dots\!\right)\dots \left(1 + \frac{1}{p_m^s} + \frac{1}{p_m^{2s}} \dots\!\right)}\\
        %Cauchyscher Multiplikationssatz
        \visible<4->{&=} \only<6->{\lim\limits_{m \to \infty}} \visible<4->{\sum_{\nu_1,\dots, \nu_m = 0}^\infty (p_1^{\nu_1}\cdots p_m^{\nu_m})^{-s}}\visible<4->{\\}
        %Eindeutigkeit der Primfaktorzerlegung
        \visible<5->{&=} \only<6->{\lim\limits_{m\to \infty}} \visible<5->{\sum_{n = p_1^{\nu_1}\cdots p_m^{\nu_m}}n^{-s}\\}
        \only<8>{\prod_{k=1}^\infty \frac{1}{1-p_k^{-s}} }\visible<7->{ &= \sum_{n=1}^\infty n^{-s}}\invisible<1->{justsomespaceforkeepingthe=}
    \end{align*}
    \end{proof}
\end{frame}
\begin{frame}
    \begin{proof}[Beweis. (Absolute Konvergenz)]
        \begin{align*}
        \sum_{k=1}^\infty \left|1 - \frac{1}{1-p_k^{-s}}\right| &= \sum_{k=1}^\infty \left|1 - \sum_{m=0}^\infty p_k^{-ms}\right|\\
        \visible<2->{&\leq \sum_{k=1}^\infty \sum_{m=1}^\infty \left| p_k^{-ms}\right|\\}
        \visible<3>{&\leq \sum_{n=1}^\infty \left|n^{-s}\right|}
        \end{align*}
    \end{proof}
\end{frame}