\begin{frame}
    \begin{block}{Beweis.}
        Absch√§tzen der Reihe ergibt
        \begin{align*}
            e^{\pi t} \cdot \sum_{n = 1}^{\infty} e^{-\pi t n^2} &= \sum_{n = 1}^{\infty} e^{-\pi t (n^2-1)}\stackrel{t \geq 1}{\leq} \sum_{n = 1}^{\infty} e^{-\pi (n^2-1)}\\
            \visible<2->{&= \sum_{n = 1}^{N} e^{-\pi (n^2-1)} + \sum_{n = N+1}^{\infty} e^{-\pi (n^2-1)}\\}
            \visible<3->{&\leq  \sum_{n = 1}^{N} e^{-\pi (n^2-1)} + \sum_{n = N+1}^{\infty} \frac{1}{n^2}\\}
            \visible<4->{&\leq B}
        \end{align*}
        \visible<5>{Also ist $\sum_{n = 1}^{\infty} e^{-\pi n^2 t} \leq B e^{-\pi t}$.}
    \end{block}
\end{frame}
\begin{frame}
    \begin{proof}
        \begin{align*}
            \int_1^\infty \sum_{n=1}^\infty e^{-\pi n^2 t} t^s \frac{\intd t}{t} &\leq B \cdot \int_1^\infty e^{-\pi t} t^{s+1} \frac{\intd t}{t^2}
            \visible<2->{\intertext{$\exists a(s):\ \forall \alpha > a: e^{-\pi \alpha} < \alpha^{-s+1}$}}
            \visible<3->{&= B \cdot \int_1^a e^{-\pi t} t^{s+1} \frac{\intd t}{t^2} + B\cdot \int_a^\infty e^{-\pi t} t^{s+1} \frac{\intd t}{t^2}\\}
            \visible<4->{&\leq B \cdot C(s) + B\cdot \int_a^\infty \frac{\intd t}{t^2}\\}
            \visible<5->{&\leq B\cdot C(s) + \frac{B}{a(s)} < \infty}
        \end{align*}
    \end{proof}
\end{frame}