\begin{frame}
\only<1>{
$(a_1, \dots, a_{n-2}) = (2,2,7,7,1,5,3,1,1,4,4,5)$\\$(b_1, \dots, b_i) = (6)$\input{cayley_animation/graph0.tex}
\hfill}
\only<2>{
$(a_1, \dots, a_{n-2}) = (2,2,7,7,1,5,3,1,1,4,4,5)$\\$(b_1, \dots, b_i) = (6,8)$\input{cayley_animation/graph1.tex}
\hfill}
\only<3>{
$(a_1, \dots, a_{n-2}) = (2,2,7,7,1,5,3,1,1,4,4,5)$\\$(b_1, \dots, b_i) = (6,8,2)$\input{cayley_animation/graph2.tex}
\hfill}
\only<4>{
$(a_1, \dots, a_{n-2}) = (2,2,7,7,1,5,3,1,1,4,4,5)$\\$(b_1, \dots, b_i) = (6,8,2,9)$\input{cayley_animation/graph3.tex}
\hfill}
\only<5>{
$(a_1, \dots, a_{n-2}) = (2,2,7,7,1,5,3,1,1,4,4,5)$\\$(b_1, \dots, b_i) = (6,8,2,9,7)$\input{cayley_animation/graph4.tex}
\hfill}
\only<6>{
$(a_1, \dots, a_{n-2}) = (2,2,7,7,1,5,3,1,1,4,4,5)$\\$(b_1, \dots, b_i) = (6,8,2,9,7,10)$\input{cayley_animation/graph5.tex}
\hfill}
\only<7>{
$(a_1, \dots, a_{n-2}) = (2,2,7,7,1,5,3,1,1,4,4,5)$\\$(b_1, \dots, b_i) = (6,8,2,9,7,10,11)$\input{cayley_animation/graph6.tex}
\hfill}
\only<8>{
$(a_1, \dots, a_{n-2}) = (2,2,7,7,1,5,3,1,1,4,4,5)$\\$(b_1, \dots, b_i) = (6,8,2,9,7,10,11,3)$\input{cayley_animation/graph7.tex}
\hfill}
\only<9>{
$(a_1, \dots, a_{n-2}) = (2,2,7,7,1,5,3,1,1,4,4,5)$\\$(b_1, \dots, b_i) = (6,8,2,9,7,10,11,3,12)$\input{cayley_animation/graph8.tex}
\hfill}
\only<10>{
$(a_1, \dots, a_{n-2}) = (2,2,7,7,1,5,3,1,1,4,4,5)$\\$(b_1, \dots, b_i) = (6,8,2,9,7,10,11,3,12,1)$\input{cayley_animation/graph9.tex}
\hfill}
\only<11>{
$(a_1, \dots, a_{n-2}) = (2,2,7,7,1,5,3,1,1,4,4,5)$\\$(b_1, \dots, b_i) = (6,8,2,9,7,10,11,3,12,1,13)$\input{cayley_animation/graph10.tex}
\hfill}
\only<12>{
$(a_1, \dots, a_{n-2}) = (2,2,7,7,1,5,3,1,1,4,4,5)$\\$(b_1, \dots, b_i) = (6,8,2,9,7,10,11,3,12,1,13,4)$\input{cayley_animation/graph11.tex}
\hfill}
\only<13>{
$(a_1, \dots, a_{n-2}) = (2,2,7,7,1,5,3,1,1,4,4,5)$\\$(b_1, \dots, b_i) = (6,8,2,9,7,10,11,3,12,1,13,4,)$\\ Die letze Kante ergibt sich aus $f_i = d_i-1$, in diesem Fall: $(5,14)$\input{cayley_animation/graph12.tex}
\hfill}
\end{frame}